src/program_proof/lockservice/rpc_logatom.v
@@ -1,0 +1,327 @@
+From Perennial.algebra Require Import auth_map.
+From Perennial.program_proof Require Import proof_prelude marshal_proof.
+From Perennial.goose_lang.lib Require Import slice.typed_slice.
+From Goose.github_com.mit_pdos.lockservice Require Import lockservice.
+From Perennial.program_proof.lockservice Require Import rpc_proof rpc nondet kv_proof fmcounter_map wpc_proofmode common_proof rpc_durable_proof.
+Require Import Decimal Ascii String DecimalString.
+From Perennial.goose_lang Require Import ffi.grove_ffi.
+
+Section rpc_logatom_proof.
+Context `{!heapG Σ}.
+Context `{!rpcG Σ u64}.
+
+
+Definition rpcReqInvUpToN_list (seqno:u64) : list coPset :=
+ ((λ (n:nat), ↑rpcRequestInvN {| Req_CID:= 0; Req_Seq:=(U64 n) |} ) <$> (seq 0 (int.nat seqno))).
+Definition rpcReqInvUpToN (seqno:u64) : coPset :=
+ ⋃ rpcReqInvUpToN_list seqno.
+
+(*
+Definition rpcReqInvUpToN (seqno:u64) : coPset :=
+  [^union list] x ∈ (seq 0 (int.nat seqno)), ↑rpcRequestInvN {| Req_CID:= 0; Req_Seq:=(U64 (Z.of_nat x)) |}. *)
+
+Lemma rpcReqInvUpToN_prop cid seq :
+  ∀ seq', int.nat seq' < int.nat seq → (↑rpcRequestInvN {|Req_CID:=cid; Req_Seq:=seq' |}) ⊆ rpcReqInvUpToN seq.
+Proof.
+  intros seq' Hineq.
+  enough (↑rpcRequestInvN {| Req_CID := cid; Req_Seq := seq' |} ∈ rpcReqInvUpToN_list seq).
+  {
+    intros x Hxin.
+    rewrite elem_of_union_list.
+    eauto.
+  }
+  unfold rpcReqInvUpToN_list.
+  eapply (elem_of_fmap_2_alt _ _ (int.nat seq')).
+  2:{
+    unfold rpcRequestInvN.
+    simpl.
+    replace (U64 (Z.of_nat (int.nat seq'))) with (seq'); first done.
+    admit.
+  }
+  admit.
+Admitted.
+
+Lemma rpcReqInvUpToN_prop_2 cid seq :
+ ∀ seq', int.nat seq' ≥ int.nat seq → ↑rpcRequestInvN {|Req_CID:=cid; Req_Seq:=seq' |} ## rpcReqInvUpToN seq.
+Admitted.
+
+
+(* Need this fupd to be OK to fire with any sequence number larger than the *)
+Definition rpc_atomic_pre_fupd γrpc (cid seq:u64) R : iProp Σ :=
+  (own γrpc.(proc) (Excl ()) -∗ cid fm[[γrpc.(lseq)]]≥ int.nat seq ={rpcReqInvUpToN seq}=∗ own γrpc.(proc) (Excl ()) ∗ R)%I.
+
+Notation "|RN={ γrpc , cid , seq }=> R" :=
+ (rpc_atomic_pre_fupd γrpc cid seq R)
+ (at level 20, right associativity)
+  : bi_scope.
+
+(* This gives the rpc_atomic_pre_fupd for any sequence number that the client can take on
+   This is the precondition for ck.MakeRequest(args), where ck has the given cid *)
+Definition rpc_atomic_pre γrpc cid R : iProp Σ :=
+    <bdisc> (∀ seq, cid fm[[γrpc.(cseq)]]↦ int.nat seq ={⊤}=∗
+    cid fm[[γrpc.(cseq)]]↦ int.nat seq ∗
+   (laterable.make_laterable (|RN={γrpc , cid , seq}=> R))).
+
+Lemma rpc_atomic_pre_fupd_mono_strong γrpc cid seq P Q:
+  (P -∗ cid fm[[γrpc.(lseq)]]≥ int.nat seq -∗
+     own γrpc.(proc) (Excl ())={rpcReqInvUpToN seq}=∗ own γrpc.(proc) (Excl ()) ∗ Q) -∗
+  |RN={γrpc,cid,seq}=> P -∗
+  |RN={γrpc,cid,seq}=> Q.
+Proof.
+  iIntros "HPQ HfupdP Hγproc #Hlb".
+  iMod ("HfupdP" with "Hγproc Hlb") as "[Hγproc HP]".
+  iSpecialize ("HPQ" with "HP Hlb Hγproc").
+  iMod "HPQ".
+  iFrame.
+  by iModIntro.
+Qed.
+
+Lemma modality_rpc_atomic_mixin γrpc cid seq :
+  modality_mixin (rpc_atomic_pre_fupd γrpc cid seq ) MIEnvId MIEnvId.
+Proof.
+  split; simpl; eauto.
+  {
+    iIntros (P) "#HP".
+    iIntros "$ _ !#".
+    done.
+  }
+  {
+    iIntros (P) "HP".
+    by iIntros "$ _ !>".
+  }
+  {
+    iIntros. iIntros "$ _".
+    by iModIntro.
+  }
+  {
+    iIntros (P Q).
+    intros HPQ.
+    iApply rpc_atomic_pre_fupd_mono_strong.
+    iIntros "HP _ $".
+    iModIntro.
+    by iApply HPQ.
+  }
+  {
+    iIntros (P Q) "[HP HQ]".
+    iIntros "Hγproc #Hlb".
+    iDestruct ("HP" with "Hγproc Hlb") as ">[Hγproc $]".
+    iDestruct ("HQ" with "Hγproc Hlb") as ">[$ $]".
+    by iModIntro.
+  }
+Qed.
+Definition modality_rpc_atomic γrpc cid seq :=
+  Modality _ (modality_rpc_atomic_mixin γrpc cid seq).
+
+(** FromModal *)
+Global Instance from_modal_rpc_atomic γrpc cid seq P :
+  FromModal (modality_rpc_atomic γrpc cid seq) (|RN={γrpc,cid,seq}=> P) (|RN={γrpc,cid,seq}=> P) P | 2.
+Proof. by rewrite /FromModal. Qed.
+
+Global Instance elim_modal_rpc_atomic γrpc cid seq' seq P Q :
+  ElimModal (int.nat seq' ≤ int.nat seq) false false (|RN={γrpc,cid,seq'}=> P) P (|RN={γrpc,cid,seq}=> Q) (|RN={γrpc,cid,seq}=> Q).
+Proof.
+  rewrite /ElimModal.
+  simpl.
+  iIntros (Hineq) "[HmodP HwandQ] Hγproc #Hlb".
+  iDestruct ("HmodP" with "Hγproc [Hlb]") as "HmodP".
+  {
+    iApply (fmcounter_map_mono_lb); last done.
+    word.
+  }
+
+  iMod (fupd_intro_mask' _ _) as "Hclose"; last iMod "HmodP" as "[Hγproc HP]".
+  {
+    admit. (* property of masks *)
+  }
+  iDestruct ("HwandQ" with "HP") as "HmodQ".
+  iMod "Hclose" as "_".
+  iDestruct ("HmodQ" with "Hγproc Hlb") as ">HmodQ".
+  iFrame.
+  by iModIntro.
+Admitted.
+
+Lemma rpc_atomic_pre_mono_strong cid γrpc P Q :
+  □(∀ seq, P -∗ |RN={γrpc,cid,seq}=> Q) -∗
+  rpc_atomic_pre γrpc cid P -∗
+  rpc_atomic_pre γrpc cid Q.
+Proof.
+  iIntros "#HPQ HatomicP".
+  iModIntro.
+  iIntros (seq) "Hcown".
+  iMod ("HatomicP" $! seq with "Hcown") as "[Hcown HatomicP]".
+  iFrame.
+  unfold laterable.make_laterable.
+  iDestruct "HatomicP" as (R) "[HR #HatomicP]".
+  iExists (R). iFrame.
+  iModIntro.
+  iModIntro.
+  iIntros "HR".
+  iMod ("HatomicP" with "HR") as "HP".
+  iDestruct ("HPQ" with "HP") as "$".
+Qed.
+
+(*
+Lemma rpc_atomic_pre_fupd_mono γrpc cid seq P Q:
+  (P -∗ Q) -∗
+  rpc_atomic_pre_fupd γrpc cid seq P -∗
+  rpc_atomic_pre_fupd γrpc cid seq Q.
+Proof.
+  iIntros "HPQ".
+  iApply rpc_atomic_pre_fupd_mono_strong.
+  iIntros "HP _ $".
+  by iApply "HPQ".
+Qed.
+
+Lemma rpc_atomic_pre_mono cid γrpc P Q :
+  <bdisc>(P -∗ Q) -∗
+  rpc_atomic_pre γrpc cid P -∗
+  rpc_atomic_pre γrpc cid Q.
+Proof.
+  iIntros "HPQ HatomicP".
+  iModIntro.
+  iIntros (seq) "Hcown".
+  iMod ("HatomicP" $! seq with "Hcown") as "[Hcown HatomicP]".
+  iFrame.
+  iApply (rpc_atomic_pre_fupd_mono with "HPQ HatomicP").
+Qed.
+*)
+
+Definition quiesce_fupd γrpc cid seqno PreCond PostCond : iProp Σ :=
+  laterable.make_laterable (rpc_atomic_pre_fupd γrpc cid seqno (▷ PreCond ∨ ▷ ∃ ret:u64, PostCond ret))%I.
+
+Definition quiesceable_pre γrpc cid PreCond PostCond : iProp Σ :=
+  rpc_atomic_pre γrpc cid (▷ PreCond ∨ ▷ ∃ ret:u64, PostCond ret)%I.
+
+Global Instance quiesceable_pre_disc γrpc cid PreCond PostCond : (Discretizable
+       (quiesceable_pre γrpc cid PreCond PostCond)).
+Proof.
+  rewrite /Discretizable.
+  by rewrite -own_discrete_idemp.
+Defined.
+
+Lemma quiesce_request (req:RPCRequestID) γrpc γreq (PreCond:iProp Σ) PostCond  :
+  is_RPCServer γrpc -∗
+  is_RPCRequest γrpc γreq PreCond PostCond req -∗
+  (RPCRequest_token γreq) -∗
+  quiesceable_pre γrpc req.(Req_CID) PreCond PostCond.
+Proof.
+    iIntros "#Hsrpc #His_req Hγpost".
+    iFrame "#∗".
+
+    iModIntro.
+
+    iIntros (new_seq) "Hcown".
+    iInv "His_req" as "[>#Hcseq_lb_strict HN]" "HNClose".
+    iMod ("HNClose" with "[$Hcseq_lb_strict $HN]") as "_".
+
+    iDestruct (fmcounter_map_agree_lb with "Hcown Hcseq_lb_strict") as %Hnew_seq.
+    iFrame.
+    iModIntro.
+    iExists (RPCRequest_token γreq).
+    iFrame.
+    iModIntro.
+    iIntros ">Hγpost".
+
+    iIntros "Hγproc #Hlseq_lb".
+    iInv "His_req" as "HN" "HNClose".
+    { apply (rpcReqInvUpToN_prop req.(Req_CID)). destruct req. simpl in *. word. }
+    iDestruct "HN" as "[#>_ [HN|HN]]"; simpl. (* Is cseq_lb_strict relevant for this? *)
+    {
+      iDestruct "HN" as "[_ [>Hbad|HN]]".
+      { iDestruct (own_valid_2 with "Hbad Hγproc") as %?; contradiction. }
+
+      iMod ("HNClose" with "[Hγpost]") as "_".
+      { iNext. iFrame "Hcseq_lb_strict". iRight. iFrame.
+        iDestruct (fmcounter_map_mono_lb (int.nat req.(Req_Seq)) with "Hlseq_lb") as "$".
+        lia.
+      }
+      iFrame.
+      iModIntro.
+      iLeft.
+      iNext.
+      iDestruct "HN" as "[_ $]".
+    }
+    {
+      iDestruct "HN" as "[#Hlseq_lb_req HN]".
+      iDestruct "HN" as "[>Hbad|Hreply_post]".
+      { by iDestruct (own_valid_2 with "Hγpost Hbad") as %Hbad. }
+      iMod ("HNClose" with "[Hγpost]") as "_".
+      {
+        iNext.
+        iFrame "Hcseq_lb_strict".
+        iRight.
+        iFrame "# ∗".
+      }
+      iDestruct "Hreply_post" as (last_reply) "[#Hreply Hpost]".
+      iModIntro.
+      iFrame.
+      iRight.
+      iExists _; iFrame.
+    }
+Qed.
+
+Lemma quiesce_idemp γrpc cid seqno Q PreCond PostCond :
+  cid fm[[γrpc.(cseq)]]≥ int.nat seqno -∗
+  □(▷Q -∗ (rpc_atomic_pre_fupd γrpc cid seqno (▷ PreCond ∨ ▷ ∃ ret:u64, PostCond ret))) -∗
+  quiesceable_pre γrpc cid Q (PostCond) -∗
+  quiesceable_pre γrpc cid PreCond PostCond.
+Proof.
+  iIntros "#Hseqno_lb #Hwand Hatomic_pre".
+  iModIntro.
+  iIntros (seq) "Hcown".
+  iDestruct (fmcounter_map_agree_lb with "Hcown Hseqno_lb") as %Hseqno_ineq.
+
+  iDestruct ("Hatomic_pre" $! seq with "Hcown") as ">[Hcown Hfupd]".
+  iFrame.
+  unfold laterable.make_laterable.
+  iDestruct "Hfupd" as (S) "[HS #Hfupd]".
+  iExists S.
+  iModIntro.
+  iFrame "HS".
+  iModIntro.
+  iIntros "HS".
+  iSpecialize ("Hfupd" with "HS").
+  iApply (rpc_atomic_pre_fupd_mono_strong with "[Hwand] Hfupd").
+  iIntros "HQR #Hlb Hγproc".
+  iDestruct (fmcounter_map_mono_lb (int.nat seqno) with "Hlb") as "#Hlb_seqno".
+  { lia. }
+  iDestruct "HQR" as "[HQ | HRpost]".
+  {
+    iDestruct ("Hwand" with "HQ") as "Hfupd".
+    iDestruct ("Hfupd" with "Hγproc Hlb_seqno") as "HH".
+    (* TODO: Show that mask of seqno is in mask of seq *)
+    (* by iModIntro. *)
+    admit.
+  }
+  { iFrame. by iModIntro. }
+Admitted.
+
+Lemma quiesce_intro γrpc cid seqno PreCond PostCond :
+  PreCond -∗ (quiesce_fupd γrpc cid seqno PreCond PostCond).
+Proof.
+  iIntros.
+  iExists (PreCond)%I.
+  iFrame.
+  iModIntro; iFrame.
+  iIntros.
+  iIntros "Hγproc #Hlb".
+  iFrame.
+    by iModIntro.
+Qed.
+
+Definition quiesce_fupd_raw γrpc cid seqno PreCond PostCond : iProp Σ :=
+  (rpc_atomic_pre_fupd γrpc cid seqno (▷ PreCond ∨ ▷ ∃ ret:u64, PostCond ret))%I.
+
+Lemma quiesceable_pre_instantiate γrpc cid seqno PreCond PostCond :
+  RPCClient_own γrpc cid seqno -∗
+  quiesceable_pre γrpc cid PreCond PostCond ={⊤}=∗
+  RPCClient_own γrpc cid seqno ∗
+  (quiesce_fupd γrpc cid seqno PreCond PostCond).
+Proof.
+  iIntros "Hcrpc Hqpre".
+  iDestruct (own_discrete_elim with "Hqpre") as "Hqpre".
+  iMod ("Hqpre" $! seqno with "Hcrpc") as "[Hcrpc Hfupd]".
+  iModIntro. iFrame.
+Qed.
+
+End rpc_logatom_proof.
